feat: final version antimono

CollapsingTowers/TwoLevelFinal/LogicalEquiv/LogicalRelation.lean
@@ -72,3 +72,361 @@ def log_approx_expr : KripkeWorld → Expr → Expr → Ty → Prop
       log_well_store 𝓦₁ σ₂ σ₃ ∧
       log_approx_value (k - j, 𝓦₁) v₀ v₁ τ
 end
+
+inductive log_approx_env : KripkeWorld → Subst → Subst → TEnv → Prop where
+  | nil : ∀ k 𝓦, log_approx_env (k, 𝓦) [] [] ⦰
+  | cons : ∀ k 𝓦 v₀ γ₀ v₁ γ₁ τ Γ,
+    log_approx_value (k, 𝓦) v₀ v₁ τ →
+    log_approx_env (k, 𝓦) γ₀ γ₁ Γ →
+    log_approx_env (k, 𝓦) (v₀ :: γ₀) (v₁ :: γ₁) ((τ, 𝟚) :: Γ)
+
+-- Γ ⊧ e₀ ≤𝑙𝑜𝑔 e₁ : τ ≜
+--   Γ ⊢ e₀ : τ ∧
+--   Γ ⊢ e₁ : τ ∧
+--   ∀ k ≥ 0, 𝓦, (k, 𝓦, γ₀, γ₁) ∈ 𝓖⟦Γ⟧. (k, 𝓦, γ₀(e₀), γ₁(e₁)) ∈ 𝓔⟦τ⟧
+@[simp]
+def log_approx (Γ : TEnv) (e₀ e₁ : Expr) (τ : Ty) : Prop :=
+  typing Γ 𝟚 e₀ τ ⊥ ∧
+  typing Γ 𝟚 e₁ τ ⊥ ∧
+  ∀ k 𝓦 γ₀ γ₁,
+    log_approx_env (k, 𝓦) γ₀ γ₁ Γ →
+    log_approx_expr (k, 𝓦) (msubst γ₀ e₀) (msubst γ₁ e₁) τ
+
+-- Γ ⊧ e₀ ≈𝑙𝑜𝑔 e₁ : τ ≜ Γ ⊧ e₀ ≤𝑙𝑜𝑔 e₁ : τ ∧ Γ ⊧ e₁ ≤𝑙𝑜𝑔 e₀ : τ
+@[simp]
+def log_equiv (Γ : TEnv) (e₀ e₁ : Expr) (τ : Ty) : Prop :=
+  log_approx Γ e₀ e₁ τ ∧ log_approx Γ e₁ e₀ τ
+
+lemma log_well_store.alloc :
+  ∀ 𝓦 σ₀ σ₁ n,
+    log_well_store 𝓦 σ₀ σ₁ →
+    log_well_store (World.ext 𝓦 σ₀.length σ₁.length) (.lit n :: σ₀) (.lit n :: σ₁) :=
+  by
+  intros 𝓦 σ₀ σ₁ n Hsem_store
+  have ⟨Hpb, Hsem_store⟩ := Hsem_store
+  constructor
+  . apply PartialBijection.ext
+    . apply Hpb
+    . intros Hdom
+      rcases Hdom with ⟨l₁, Hrel⟩
+      have ⟨n, Hbinds₀, Hbinds₁⟩ := Hsem_store _ _ Hrel
+      have _ := (getr_exists_iff_index_lt_length σ₀ σ₀.length).mpr (by exists .lit n)
+      omega
+    . intros Hrange
+      rcases Hrange with ⟨l₀, Hrel⟩
+      have ⟨n, Hbinds₀, Hbinds₁⟩ := Hsem_store _ _ Hrel
+      have _ := (getr_exists_iff_index_lt_length σ₁ σ₁.length).mpr (by exists .lit n)
+      omega
+  . intros l₀ l₁ Hrel
+    cases Hrel
+    case inl HEq => simp [HEq]
+    case inr Hrel =>
+      have ⟨n, Hbinds₀, Hbinds₁⟩ := Hsem_store _ _ Hrel
+      exists n; constructor
+      . apply binds.extend _ [_] _ _ Hbinds₀
+      . apply binds.extend _ [_] _ _ Hbinds₁
+
+lemma log_well_store.store :
+  ∀ 𝓦 l₀ l₁ σ₀ σ₁ σ₂ σ₃ n,
+    log_well_store 𝓦 σ₀ σ₁ →
+    𝓦 l₀ l₁ →
+    patch l₀ (.lit n) σ₀ σ₂ →
+    patch l₁ (.lit n) σ₁ σ₃ →
+    log_well_store 𝓦 σ₂ σ₃ :=
+  by
+  intros 𝓦 l₀ l₁ σ₀ σ₁ σ₂ σ₃ n Hsem_store Hrel₀ Hpatch₀ Hpatch₁
+  have ⟨Hpb, Hsem_store⟩ := Hsem_store
+  constructor
+  . apply Hpb
+  . intros l₂ l₃ Hrel₁
+    cases (PartialBijection.eq_or_disjoint _ _ _ _ _ Hpb Hrel₀ Hrel₁)
+    case inl HEq =>
+      simp [← HEq]
+      exists n; constructor
+      . apply patch.binds_eq _ _ _ _ Hpatch₀
+      . apply patch.binds_eq _ _ _ _ Hpatch₁
+    case inr HNe =>
+      have ⟨n, Hbinds₀, Hbinds₁⟩ := Hsem_store _ _ Hrel₁
+      exists n; constructor
+      . apply patch.binds_disjoint _ _ _ _ _ _ Hpatch₀ HNe.left Hbinds₀
+      . apply patch.binds_disjoint _ _ _ _ _ _ Hpatch₁ HNe.right Hbinds₁
+
+lemma log_approx_value.antimono :
+  ∀ k₀ k₁ 𝓦₀ 𝓦₁ v₀ v₁ τ,
+    log_approx_value (k₀, 𝓦₀) v₀ v₁ τ →
+    ((k₁, 𝓦₁) ⊇ (k₀, 𝓦₀)) →
+    log_approx_value (k₁, 𝓦₁) v₀ v₁ τ :=
+  by
+  intros k₀ k₁ 𝓦₀ 𝓦₁ v₀ v₁ τ Hsem_value Hfuture₀
+  cases τ
+  case nat =>
+    cases v₀ <;> try simp at Hsem_value
+    case lit n₀ =>
+    cases v₁ <;> try simp at Hsem_value
+    case lit n₁ =>
+    simp; apply Hsem_value
+  case arrow τ𝕒 τ𝕓 φ =>
+    cases v₀ <;> try simp at Hsem_value
+    case lam e₀ =>
+    cases v₁ <;> try simp at Hsem_value
+    case lam e₁ =>
+    cases φ <;> simp only [log_approx_value] at Hsem_value <;> try contradiction
+    have ⟨Hwf₀, HG₀, Hwf₁, HG₁, Hsem_value⟩ := Hsem_value
+    simp only [log_approx_value]
+    constructor; apply Hwf₀
+    constructor; apply HG₀
+    constructor; apply Hwf₁
+    constructor; apply HG₁
+    intros k₂ 𝓦₂ v₀ v₁ Hfuture₁
+    apply Hsem_value
+    have ⟨Hk₀, Hfuture₀⟩ := Hfuture₀
+    have ⟨Hk₁, Hfuture₁⟩ := Hfuture₁
+    constructor
+    . omega
+    . apply World.future.trans _ _ _ Hfuture₁
+      apply Hfuture₀
+  case unit =>
+    cases v₀ <;> try simp at Hsem_value
+    case unit =>
+    cases v₁ <;> try simp at Hsem_value
+    case unit =>
+    simp
+  case ref τ =>
+    cases v₀ <;> try simp at Hsem_value
+    case loc l₀ =>
+    cases v₁ <;> try simp at Hsem_value
+    case loc l₁ =>
+    cases τ <;> simp only [log_approx_value] at Hsem_value <;> try contradiction
+    simp only [log_approx_value]
+    apply Hfuture₀.right; apply Hsem_value
+  case fragment => simp at Hsem_value
+  case rep => simp at Hsem_value
+
+lemma log_approx_env.antimono :
+  ∀ k₀ k₁ 𝓦₀ 𝓦₁ γ₀ γ₁ Γ,
+    log_approx_env (k₀, 𝓦₀) γ₀ γ₁ Γ →
+    ((k₁, 𝓦₁) ⊇ (k₀, 𝓦₀)) →
+    log_approx_env (k₁, 𝓦₁) γ₀ γ₁ Γ :=
+  by
+  intros k₀ k₁ 𝓦₀ 𝓦₁ γ₀ γ₁ Γ HsemΓ Hfuture
+  generalize HEqi𝓦₀ : (k₀, 𝓦₀) = i𝓦₀
+  rw [HEqi𝓦₀] at HsemΓ
+  induction HsemΓ
+  case nil => apply log_approx_env.nil
+  case cons Hsem_value _ IH =>
+    rw [← HEqi𝓦₀] at Hsem_value
+    apply log_approx_env.cons
+    apply log_approx_value.antimono; apply Hsem_value; apply Hfuture
+    apply IH; apply HEqi𝓦₀
+
+lemma log_approx_value.syntactic.value :
+  ∀ k 𝓦 v₀ v₁ τ,
+    log_approx_value (k, 𝓦) v₀ v₁ τ →
+    value v₀ ∧ value v₁ :=
+  by
+  intros k 𝓦 v₀ v₁ τ Hsem_value
+  cases τ
+  case nat =>
+    cases v₀ <;> try simp at Hsem_value
+    case lit n₀ =>
+    cases v₁ <;> try simp at Hsem_value
+    case lit n₁ =>
+    constructor
+    apply value.lit
+    apply value.lit
+  case unit =>
+    cases v₀ <;> try simp at Hsem_value
+    case unit =>
+    cases v₁ <;> try simp at Hsem_value
+    case unit =>
+    constructor
+    apply value.unit
+    apply value.unit
+  case arrow τ𝕒 τ𝕓 φ =>
+    cases v₀ <;> try simp at Hsem_value
+    case lam e₀ =>
+    cases v₁ <;> try simp at Hsem_value
+    case lam e₁ =>
+    cases φ <;> simp only [log_approx_value] at Hsem_value <;> try contradiction
+    have ⟨Hwf₀, HG₀, Hwf₁, HG₁, Hsem_value⟩ := Hsem_value
+    constructor
+    apply value.lam; apply Hwf₀.left
+    apply value.lam; apply Hwf₁.left
+  case ref τ =>
+    cases v₀ <;> try simp at Hsem_value
+    case loc l₀ =>
+    cases v₁ <;> try simp at Hsem_value
+    case loc l₁ =>
+    cases τ <;> simp only [log_approx_value] at Hsem_value <;> try contradiction
+    constructor
+    apply value.loc
+    apply value.loc
+  case fragment => simp at Hsem_value
+  case rep => simp at Hsem_value
+
+lemma log_approx_value.syntactic.wf :
+  ∀ k 𝓦 v₀ v₁ τ,
+    log_approx_value (k, 𝓦) v₀ v₁ τ →
+    wf v₀ ∧ wf v₁ :=
+  by
+  intros k 𝓦 v₀ v₁ τ Hsem_value
+  cases τ
+  case nat =>
+    cases v₀ <;> try simp at Hsem_value
+    case lit n₀ =>
+    cases v₁ <;> try simp at Hsem_value
+    case lit n₁ =>
+    simp
+  case arrow τ𝕒 τ𝕓 φ =>
+    cases v₀ <;> try simp at Hsem_value
+    case lam e₀ =>
+    cases v₁ <;> try simp at Hsem_value
+    case lam e₁ =>
+    cases φ <;> simp only [log_approx_value] at Hsem_value <;> try contradiction
+    have ⟨Hwf₀, HG₀, Hwf₁, HG₁, Hsem_value⟩ := Hsem_value
+    constructor
+    apply Hwf₀
+    apply Hwf₁
+  case unit =>
+    cases v₀ <;> try simp at Hsem_value
+    case unit =>
+    cases v₁ <;> try simp at Hsem_value
+    case unit =>
+    simp
+  case ref τ =>
+    cases v₀ <;> try simp at Hsem_value
+    case loc l₀ =>
+    cases v₁ <;> try simp at Hsem_value
+    case loc l₁ =>
+    cases τ <;> simp only [log_approx_value] at Hsem_value <;> try contradiction
+    simp
+  case fragment => simp at Hsem_value
+  case rep => simp at Hsem_value
+
+lemma log_approx_value.syntactic.grounded :
+  ∀ k 𝓦 v₀ v₁ τ,
+    log_approx_value (k, 𝓦) v₀ v₁ τ →
+    grounded v₀ ∧ grounded v₁ :=
+  by
+  intros k 𝓦 v₀ v₁ τ Hsem_value
+  cases τ
+  case nat =>
+    cases v₀ <;> try simp at Hsem_value
+    case lit n₀ =>
+    cases v₁ <;> try simp at Hsem_value
+    case lit n₁ =>
+    simp
+  case arrow τ𝕒 τ𝕓 φ =>
+    cases v₀ <;> try simp at Hsem_value
+    case lam e₀ =>
+    cases v₁ <;> try simp at Hsem_value
+    case lam e₁ =>
+    cases φ <;> simp only [log_approx_value] at Hsem_value <;> try contradiction
+    have ⟨Hwf₀, HG₀, Hwf₁, HG₁, Hsem_value⟩ := Hsem_value
+    constructor
+    apply HG₀
+    apply HG₁
+  case unit =>
+    cases v₀ <;> try simp at Hsem_value
+    case unit =>
+    cases v₁ <;> try simp at Hsem_value
+    case unit =>
+    simp
+  case ref τ =>
+    cases v₀ <;> try simp at Hsem_value
+    case loc l₀ =>
+    cases v₁ <;> try simp at Hsem_value
+    case loc l₁ =>
+    cases τ <;> simp only [log_approx_value] at Hsem_value <;> try contradiction
+    simp
+  case fragment => simp at Hsem_value
+  case rep => simp at Hsem_value
+
+lemma log_approx_value.apply :
+  ∀ k 𝓦 f₀ arg₀ f₁ arg₁ τ𝕒 τ𝕓,
+    log_approx_value (k, 𝓦) f₀ f₁ (.arrow τ𝕒 τ𝕓 ⊥) →
+    log_approx_value (k, 𝓦) arg₀ arg₁ τ𝕒 →
+    log_approx_expr (k, 𝓦) (.app₁ f₀ arg₀) (.app₁ f₁ arg₁) τ𝕓 :=
+  by
+  intros k 𝓦 f₀ arg₀ f₁ arg₁ τ𝕒 τ𝕓 Hsem_value_fun Hsem_value_arg
+  cases f₀ <;> cases f₁ <;> simp only [log_approx_value] at Hsem_value_fun <;> try contradiction
+  have ⟨_, _, _, _, Hsem_value_fun⟩ := Hsem_value_fun
+  apply Hsem_value_fun
+  constructor; omega; apply World.future.refl
+  apply Hsem_value_arg
+
+lemma log_approx_env.length :
+  ∀ k 𝓦 γ₀ γ₁ Γ,
+    log_approx_env (k, 𝓦) γ₀ γ₁ Γ →
+    γ₀.length = Γ.length ∧
+    γ₁.length = Γ.length :=
+  by
+  intros k 𝓦 γ₀ γ₁ Γ H
+  generalize HEqi𝓦 : (k, 𝓦) = i𝓦
+  rw [HEqi𝓦] at H
+  induction H
+  case nil => simp
+  case cons IH =>
+    constructor
+    . simp; apply (IH HEqi𝓦).left
+    . simp; apply (IH HEqi𝓦).right
+
+lemma log_approx_env.binds_log_approx_value :
+  ∀ k 𝓦 γ₀ γ₁ Γ x τ,
+    log_approx_env (k, 𝓦) γ₀ γ₁ Γ →
+    binds x (τ, 𝟚) Γ →
+    log_approx_value (k, 𝓦) (msubst γ₀ (.fvar x)) (msubst γ₁ (.fvar x)) τ :=
+  by
+  intros k 𝓦 γ₀ γ₁ Γ x τ HsemΓ Hbinds
+  generalize HEqi𝓦 : (k, 𝓦) = i𝓦
+  rw [HEqi𝓦] at HsemΓ
+  induction HsemΓ
+  case nil => nomatch Hbinds
+  case cons v₀ γ₀ v₁ γ₁ τ Γ Hsem_value HsemΓ IH =>
+    have ⟨Hwf₀, Hwf₁⟩ := log_approx_value.syntactic.wf _ _ _ _ _ Hsem_value
+    have ⟨HEq₀, HEq₁⟩ := log_approx_env.length _ _ _ _ _ HsemΓ
+    simp [HEq₀, HEq₁]
+    by_cases HEqx : Γ.length = x
+    . simp [if_pos HEqx]
+      simp [if_pos HEqx] at Hbinds
+      rw [← Hbinds, identity.msubst, identity.msubst]
+      apply Hsem_value
+      apply Hwf₁.right
+      apply Hwf₀.right
+    . simp [if_neg HEqx]
+      simp [if_neg HEqx] at Hbinds
+      apply IH; apply Hbinds; apply HEqi𝓦
+
+lemma log_approx_env.syntactic.mwf :
+  ∀ k 𝓦 γ₀ γ₁ Γ,
+    log_approx_env (k, 𝓦) γ₀ γ₁ Γ →
+    mwf γ₀ ∧ mwf γ₁ :=
+  by
+  intros k 𝓦 γ₀ γ₁ Γ HsemΓ
+  generalize HEqi𝓦 : (k, 𝓦) = i𝓦
+  rw [HEqi𝓦] at HsemΓ
+  induction HsemΓ
+  case nil => simp
+  case cons v₀ γ₀ v₁ γ₁ τ Γ Hsem_value HsemΓ IH =>
+    have ⟨IH₀, IH₁⟩ := IH HEqi𝓦
+    have ⟨H₀, H₁⟩ := log_approx_value.syntactic.wf _ _ _ _ _ Hsem_value
+    constructor
+    . exact ⟨H₀, IH₀⟩
+    . exact ⟨H₁, IH₁⟩
+
+lemma log_approx_env.syntactic.mgrounded :
+  ∀ k 𝓦 γ₀ γ₁ Γ,
+    log_approx_env (k, 𝓦) γ₀ γ₁ Γ →
+    mgrounded γ₀ ∧ mgrounded γ₁ :=
+  by
+  intros k 𝓦 γ₀ γ₁ Γ HsemΓ
+  generalize HEqi𝓦 : (k, 𝓦) = i𝓦
+  rw [HEqi𝓦] at HsemΓ
+  induction HsemΓ
+  case nil => simp
+  case cons v₀ γ₀ v₁ γ₁ τ Γ Hsem_value HsemΓ IH =>
+    have ⟨IH₀, IH₁⟩ := IH HEqi𝓦
+    have ⟨H₀, H₁⟩ := log_approx_value.syntactic.grounded _ _ _ _ _ Hsem_value
+    constructor
+    . exact ⟨H₀, IH₀⟩
+    . exact ⟨H₁, IH₁⟩
